theories/logic/ewp_wrp.v
@@ -1,0 +1,391 @@
+(* ewp_wrp.v *)
+
+From iris.proofmode Require Import base tactics.
+From iris.algebra Require Import ofe list.
+From iris.base_logic Require Export iprop upred invariants.
+
+(* Hazel Reasoning *)
+From hazel.program_logic Require Import weakest_precondition 
+                                        basic_reasoning_rules
+                                        state_reasoning
+                                        shallow_handler_reasoning
+                                        deep_handler_reasoning
+                                        tactics
+                                        protocols.
+
+(* Local imports *)
+From haffel.lib Require Import logic.
+From haffel.lang Require Import hazel.
+From haffel.lang Require Import subst_map.
+From haffel.logic Require Import iEff.
+From haffel.logic Require Import sem_def.
+From haffel.logic Require Import sem_sig.
+
+(* EWP wrapper *)
+Definition ewp_wrp `{!heapGS Σ} (E : coPset) (e : expr) (σ : sem_sig Σ) (Φ : val -d> iPropO Σ) : iPropO Σ := 
+  (match σ.1 with
+    OS => EWP e @ E <| σ.2 |> {| σ.2 |} {{ Φ }}
+  | MS => EWP e @ E <| ⊥ |>   {| σ.2 |} {{ Φ }}
+  end)%I.
+
+Global Opaque env_dom.
+
+Notation "'EWPW' e @ E {{ Φ } }" :=
+  (ewp_wrp E e%E ⊥ Φ)
+  (at level 20, e, Φ at level 200,
+   format "'[' 'EWPW'  e  '/' '[          ' @  E  {{  Φ  } } ']' ']'") : bi_scope.
+
+(* Postcondition includes binder. *)
+Notation "'EWPW' e @ E {{ v , Φ } }" :=
+  (ewp_wrp E e%E ⊥ (λ v, Φ)%I)
+  (at level 20, e, Φ at level 200,
+   format "'[' 'EWPW'  e  '/' '[          ' @  E  {{  v ,  Φ  } } ']' ']'") : bi_scope.
+
+(* Mask is implicitly specified by ⊤. *)
+Notation "'EWPW' e {{ v , Φ } }" :=
+  (ewp_wrp ⊤ e%E ⊥ (λ v, Φ)%I)
+  (at level 20, e, Φ at level 200,
+   format "'[' 'EWPW'  e  '/' '[          ' {{  v ,  Φ  } } ']' ']'") : bi_scope.
+
+(* No binder and no mask. *)
+Notation "'EWPW' e {{ Φ } }" :=
+  (ewp_def ⊤ e%E ⊥ Φ%I)
+  (at level 20, e, Φ at level 200,
+   format "'[' 'EWPW'  e  '/' '[          ' {{  Φ  } } ']' ']'") : bi_scope.
+
+Notation "'EWPW' e @ E '<|' σ '|' '>' {{ Φ } }" :=
+  (ewp_wrp E e%E σ Φ)
+  (at level 20, e, σ, Φ at level 200,
+   format "'[' 'EWPW'  e  '/' '[          ' @  E '<|' σ '|' '>' {{  Φ  } } ']' ']'") : bi_scope.
+
+(* Postcondition includes binder. *)
+Notation "'EWPW' e @ E '<|' σ '|' '>' {{ v , Φ } }" :=
+  (ewp_wrp E e%E σ (λ v, Φ)%I)
+  (at level 20, e, σ, Φ at level 200,
+   format "'[' 'EWPW'  e  '/' '[          ' @  E '<|' σ '|' '>'  {{  v ,  Φ  } } ']' ']'") : bi_scope.
+
+(* Mask is implicitly specified by ⊤. *)
+Notation "'EWPW' e '<|' σ '|' '>' {{ v , Φ } }" :=
+  (ewp_wrp ⊤ e%E σ (λ v, Φ)%I)
+  (at level 20, e, σ, Φ at level 200,
+   format "'[' 'EWPW'  e  '/' '[          ' '<|' σ '|' '>' {{  v ,  Φ  } } ']' ']'") : bi_scope.
+
+(* No binder and no mask. *)
+Notation "'EWPW' e '<|' σ '|' '>' {{ Φ } }" :=
+  (ewp_wrp ⊤ e%E σ Φ%I)
+  (at level 20, e, σ, Φ at level 200,
+   format "'[' 'EWPW'  e  '/' '[          ' '<|' σ '|' '>' {{  Φ  } } ']' ']'") : bi_scope.
+
+Global Instance ewp_wrp_ne `{!heapGS Σ} E e σ : 
+  NonExpansive (ewp_wrp E e σ).
+Proof.
+  rewrite /ewp_wrp. intros ????. by repeat f_equiv.
+Qed.
+
+Global Instance ewp_wrp_contractive `{!heapGS Σ} E e σ : 
+  TCEq (to_val e) None →
+  TCEq (to_eff e) None →
+  Contractive (ewp_wrp E e σ).
+Proof.
+  rewrite /ewp_wrp. intros ??????. 
+  f_equiv; by f_contractive. 
+Qed.
+
+Definition is_os `{!heapGS Σ} (σ : sem_sig Σ) := (
+    (σ ≤S ⊥) ∨ 
+      (∃ τ κ, ⌜ NonExpansive2 τ ⌝ ∗ ⌜ NonExpansive2 κ ⌝ ∗
+              (σ ≤S (μ∀TS: θ, α, τ θ α ⇒ κ θ α | OS)%S) ∗ 
+              ((μ∀TS: θ, α, τ θ α ⇒ κ θ α | OS)%S ≤S σ))
+)%I. 
+
+Section reasoning.
+
+  Context `{!heapGS Σ}. 
+
+  Lemma bot_is_os : ⊢ is_os ⊥.
+  Proof. iLeft. iApply sig_le_refl. Qed.
+  
+  Lemma os_is_os A B `{ NonExpansive2 A, NonExpansive2 B} : 
+    ⊢ is_os (μ∀TS: θ, α, A θ α ⇒ B θ α | OS)%S.
+  Proof. 
+    iRight. iExists A, B. 
+    do 2 (iSplit; first done).
+    iSplit; iApply sig_le_refl. 
+  Qed.
+  
+  Lemma ewpw_ewp_eq E e σ (Φ : val -d> iProp Σ) :
+    (EWPW e @ E <| σ |> {{ Φ }})%I = (EWP e @E <| match σ.1 with OS => σ.2 | MS => ⊥ end |> {| σ.2 |} {{ Φ }})%I.
+  Proof. rewrite /ewp_wrp. by destruct σ.1. Qed.
+
+  Lemma ewp_wrp_value (E : coPset) σ Φ (v : val) :
+    Φ v -∗ EWPW v @E <| σ |> {{ Φ }}.
+  Proof.
+    iIntros "HΦ". rewrite /ewp_wrp. destruct σ.1; by iApply ewp_value. 
+  Qed.
+  
+  Lemma ewp_wrp_bot E e Φ :
+    EWP e @ E {{ v, Φ v }} -∗
+    EWPW e @ E {{ Φ }}.
+  Proof. iIntros "Hewp". by rewrite /ewp_wrp. Qed.
+  
+  Lemma ewp_wrp_bot_inv e E Φ :
+    EWPW e @ E {{ Φ }} -∗
+    EWP e @ E {{ v, Φ v }}.
+  Proof. by iIntros "Hewp". Qed.
+  
+  Lemma ewp_sem_os_sig_le_sub E σ σ' e Φ :
+    σ ≤S σ' -∗
+    EWP e @ E <| σ.2 |> {| σ.2 |} {{ v, Φ v }} -∗
+    EWP e @ E <| σ'.2 |> {| σ'.2 |} {{ v, Φ v }}.
+  Proof.
+    iIntros "[#Hbot|[#Hmle #Hple]] Hewp".
+    - iApply ewp_ms_prot_mono; first iApply iEff_le_bottom.
+      iApply ewp_os_prot_mono; first iApply iEff_le_bottom.
+      iDestruct (ewp_ms_prot_mono with "Hbot Hewp") as "Hewp".
+      by iDestruct (ewp_os_prot_mono with "Hbot Hewp") as "Hewp".
+    - iApply ewp_ms_prot_mono; first iApply "Hple".
+      by iApply ewp_os_prot_mono; first iApply "Hple".
+  Qed.
+  
+  Lemma ewp_sem_ms_sig_le_sub E σ σ' e Φ :
+    σ ≤S σ' -∗
+    EWP e @ E <| ⊥ |> {| σ.2 |} {{ v, Φ v }} -∗
+    EWP e @ E <| ⊥ |> {| σ'.2 |} {{ v, Φ v }}.
+  Proof.
+    iIntros "[#Hbot|[#Hmle #Hple]] Hewp".
+    - iApply ewp_ms_prot_mono; first iApply iEff_le_bottom.
+      by iDestruct (ewp_ms_prot_mono with "Hbot Hewp") as "Hewp".
+    - by iApply ewp_ms_prot_mono; first iApply "Hple".
+  Qed.
+  
+  Lemma ewp_wrp_sub E e σ σ' Φ :
+    σ ≤S σ' -∗ 
+    EWPW e @E <| σ |> {{ Φ }} -∗ EWPW e @E <| σ' |> {{ Φ }}. 
+  Proof.
+    iIntros "#Hσσ' Hewp". 
+    iDestruct "Hσσ'" as "[Hbot|[Hmle Hple]]".
+    - rewrite /ewp_wrp; destruct σ.1,σ'.1;
+      (iApply ewp_ms_prot_mono; first iApply iEff_le_bottom);
+      (iApply ewp_os_prot_mono; first iApply iEff_le_bottom);
+      iDestruct (ewp_ms_prot_mono with "Hbot Hewp") as "Hewp";
+      by try iDestruct (ewp_os_prot_mono with "Hbot Hewp") as "Hewp".
+    - rewrite /ewp_wrp. destruct σ.1 eqn:H1, σ'.1 eqn:H2; 
+      rewrite /mode_le /mode_le_prop; eauto.
+      + iApply ewp_ms_prot_mono; first iApply "Hple".
+        by iApply ewp_os_prot_mono; first iApply "Hple".
+      + iApply ewp_ms_prot_mono; first iApply "Hple".
+        by iApply ewp_os_prot_mono; first iApply iEff_le_bottom.
+      + iApply ewp_ms_prot_mono; first iApply "Hple".
+        by iApply ewp_os_prot_mono; first iApply iEff_le_bottom.
+  Qed.
+  
+  Lemma ewp_mono_os E σ σ' e Φ Φ' :
+    is_os σ -∗ is_os σ' -∗
+    EWP e @ E <| σ.2 |> {| σ'.2 |} {{ v, Φ v }} -∗
+    (∀ v : val, Φ v ={E}=∗ Φ' v) -∗ EWP e @ E <| σ.2 |> {| σ'.2 |} {{ v, Φ' v }}.
+  Proof.
+    iIntros "#HOS #HOS' Hewp Himp". 
+    iLöb as "IH" forall (e).
+    rewrite !ewp_unfold /ewp_pre.
+    destruct (to_val e) eqn:?.
+    { iMod "Hewp" as "Hewp". by iApply "Himp". }
+    destruct (to_eff e) eqn:?.
+    - simpl. destruct p eqn:?, p0 eqn:?, m;
+      iDestruct "Hewp" as "(%Φ'' & HΨ & Hps)"; 
+      iExists (λ w, Φ'' w ∗ (∀ v, Φ v ={E}=∗ Φ' v)%I)%I;
+      iSplitL "HΨ Himp".
+      2, 4: try (iDestruct "Hps" as "#Hps"; iModIntro);
+            iIntros "% (HΦ'' & Himp)"; 
+            iSpecialize ("Hps" with "HΦ''"); iNext;
+            iApply ("IH" with "Hps Himp").
+      + iDestruct "HOS" as "[Hbot|Hple]".
+        { iDestruct (sem_sig_bot_ieff with "Hbot HΨ") as "[]". }
+        iDestruct "Hple" as "(%κ & %τ & %Hneτ & %Hneκ & Hle1 & Hle2)".
+        iDestruct (sem_sig_to_ieff with "Hle1 HΨ") as "HΨ".
+        iApply (sem_sig_to_ieff with "Hle2"). 
+        rewrite !sem_sig_eff_rec_eq.
+        iDestruct "HΨ" as "(%α & %u & Hrw & HA & HPost)".
+        iExists α, u. iFrame. simpl.
+        iIntros (b) "HB". iFrame. by iApply "HPost".
+      + iDestruct "HOS'" as "[Hbot|Hple]".
+        { iDestruct (sem_sig_bot_ieff with "Hbot HΨ") as "[]". }
+        iDestruct "Hple" as "(%κ & %τ & %Hneτ & %Hneκ & Hle1 & Hle2)".
+        iDestruct (sem_sig_to_ieff with "Hle1 HΨ") as "HΨ".
+        iApply (sem_sig_to_ieff with "Hle2"). 
+        rewrite !sem_sig_eff_rec_eq.
+        iDestruct "HΨ" as "(%α & %u & Hrw & HA & HPost)".
+        iExists α, u. iFrame. simpl.
+        iIntros (b) "HB". iFrame. by iApply "HPost".
+    - iIntros (σ₁ ns κ' κs nt) "Hstate".
+      iSpecialize ("Hewp" $! σ₁ ns κ' κs nt with "Hstate"). 
+      iMod "Hewp" as "Hewp". iModIntro.
+      iDestruct "Hewp" as "(Hred & Hpost)".
+      iFrame. iIntros (e₂ σ₂) "Hprim Hcred".
+      iSpecialize ("Hpost" $! e₂ σ₂ with "Hprim Hcred").
+      iInduction (num_laters_per_step) as [|] "IH'"; simpl.
+      { iMod "Hpost" as "Hpost". iModIntro. iNext.
+        do 2 (iMod "Hpost" as "Hpost"; iModIntro).
+        iDestruct "Hpost" as "[$ He₂]".
+        iApply ("IH" with "He₂ Himp" ). }
+      iMod "Hpost" as "Hpost". iModIntro. iNext.
+      iMod "Hpost" as "Hpost". iClear "IH".
+      iMod ("IH'" with "Hpost Himp") as "IH".
+      do 2 iModIntro. iNext. iApply "IH".
+  Qed.
+  
+  Lemma ewp_wrp_mono_os E σ e Φ Φ' :
+    is_os σ -∗
+    EWPW e @ E <| σ |> {{ Φ }} -∗
+    (∀ v : val, Φ v ={E}=∗ Φ' v) -∗ 
+    EWPW e @E <| σ |> {{ Φ' }}. 
+  Proof.
+    iIntros "#HOS Hewp HΦ". rewrite /ewp_wrp. destruct σ.1. 
+    { iApply (ewp_mono_os with "HOS HOS Hewp HΦ"). }
+    iApply (ewp_mono_os _ ⊥ with "[] HOS [Hewp] HΦ"); [iLeft; iApply sig_le_nil|done].
+  Qed.
+  
+  Lemma ewp_wrp_mono E σ e Φ Φ' :
+    EWPW e @E <| σ |> {{ Φ }} -∗
+    □ (∀ v : val, Φ v ={E}=∗ Φ' v) -∗ 
+    EWPW e @E <| σ |> {{ Φ' }}.
+  Proof.
+    iIntros "Hewp HΦ". rewrite /ewp_wrp. destruct σ.1; 
+    iApply (ewp_pers_mono with "Hewp HΦ").
+  Qed.
+  
+  Lemma ewp_wrp_pure_step' E e e' σ Φ :
+    pure_prim_step e e' → 
+    ▷ EWPW e' @E <| σ |>  {{ Φ }} -∗
+    EWPW e @E <| σ |> {{ Φ }}. 
+  Proof.
+    iIntros "%Hprim Hewp". rewrite /ewp_wrp. 
+    destruct σ.1; by iApply ewp_pure_step'.
+  Qed.
+  
+  Lemma ewp_wrp_bind k `{NeutralEctx k} E σ e e' Φ  :
+    e' = fill k e →
+    EWPW e @E <| σ |> {{ w, EWPW (fill k w) @E <| σ |> {{ Φ }} }} -∗
+    EWPW e' @E <| σ |> {{ Φ }}.
+  Proof.
+    iIntros (?) "Hewp". rewrite /ewp_wrp. destruct σ.1;
+    by iApply ewp_bind.
+  Qed.
+  
+  Lemma ewp_wrp_alloc E σ Φ v :
+    ▷ (∀ (l : loc), l ↦ v ={E}=∗ Φ #l) -∗
+      EWPW (ref v)%E @E <| σ |> {{ Φ }}.
+  Proof.
+    iIntros "H". rewrite /ewp_wrp. destruct σ.1; by iApply ewp_alloc. 
+  Qed.
+  
+  Lemma ewp_wrp_load E σ Φ l q v :
+    ▷ l ↦{q} v -∗
+      ▷ (l ↦{q} v ={E}=∗ Φ v) -∗
+        EWPW (Load #l)%E @E <| σ |> {{ Φ }}.
+  Proof.
+    iIntros "H". rewrite /ewp_wrp. destruct σ.1; by iApply ewp_load. 
+  Qed.
+  
+  Lemma ewp_wrp_store E σ Φ l v w :
+    ▷ l ↦ v -∗
+      ▷ (l ↦ w ={E}=∗ Φ #()) -∗
+        EWPW (#l <- w)%E @E <| σ |> {{ Φ }}.
+  Proof.
+    iIntros "H". rewrite /ewp_wrp. destruct σ.1; by iApply ewp_store. 
+  Qed.
+  
+  Lemma ewp_wrp_replace E σ Φ l v w :
+    ▷ l ↦ v -∗
+      ▷ (l ↦ w ={E}=∗ Φ v) -∗
+        EWPW (#l <!- w)%E @E <| σ |> {{ Φ }}.
+  Proof.
+    iIntros "H". rewrite /ewp_wrp. destruct σ.1; by iApply ewp_replace. 
+  Qed.
+  
+  Lemma ewp_wrp_free E σ Φ l v :
+    ▷ l ↦ v -∗
+      ▷ (|={E}=> Φ v) -∗
+        EWPW (Free #l)%E @E <| σ |> {{ Φ }}.
+  Proof.
+    iIntros "H". rewrite /ewp_wrp. destruct σ.1; by iApply ewp_free. 
+  Qed.
+  
+  Lemma ewp_wrp_atomic E1 E2 e σ Φ `{!Atomic StronglyAtomic e} :
+    TCEq (to_eff e) None →
+      (|={E1,E2}=> EWPW e @E2 <| σ |> {{ v, |={E2,E1}=> Φ v }}) -∗
+        EWPW e @E1 <| σ |> {{ Φ }}.
+  Proof.
+    iIntros (?) "H". rewrite /ewp_wrp. destruct σ.1; by iApply ewp_atomic. 
+  Qed.
+
+  Lemma ewp_wrp_eff_os E σ Φ v k :
+    iEff_car (upcl OS σ) v (λ w, ▷ EWPW (fill k (Val w)) @ E <| (OS, σ) |> {{ Φ }}) -∗
+    EWPW (of_eff OS v k) @ E <| (OS, σ) |> {{ Φ }}.
+  Proof. 
+    iIntros "H". rewrite /ewp_wrp /=.
+    by iApply ewp_eff_os.
+  Qed.
+
+  Lemma ewp_wrp_do_os E v σ Φ :
+    σ.1 ≡ OS -∗
+    iEff_car σ.2 v Φ -∗ EWPW (do: v) @ E <| σ |> {{ Φ }}.
+  Proof.
+    iIntros "HOS Hσ".
+    rewrite /ewp_wrp /=. 
+    destruct σ.1 eqn:H; rewrite H; 
+    last (iDestruct "HOS" as "%HOS"; discriminate).
+    iApply ewp_do_os.
+    simpl. iExists Φ. iFrame. iIntros (w) "$".
+  Qed.
+
+  Lemma ewp_wrp_do_ms E v σ Φ :
+    iEff_car σ.2 v Φ -∗ EWPW (doₘ: v) @ E <| σ |> {{ Φ }}.
+  Proof.
+    iIntros "Hσ".
+    rewrite /ewp_wrp /=. 
+    destruct σ.1 eqn:H; iApply ewp_do_ms;
+    simpl; iExists Φ; iFrame; iIntros "!# % $".
+  Qed.
+
+  Definition shallow_handler_wrp
+  (E : coPset)
+  (σ : sem_sig Σ)
+  (Φ : val -d> iProp Σ)
+  (h r : expr)
+  (σ' : sem_sig Σ)
+  (Φ' : val -d> iProp Σ) : iProp Σ :=
+    shallow_handler E (match σ.1 with OS => σ.2 | MS => ⊥ end) σ.2 Φ h r
+                      (match σ'.1 with OS => σ'.2 | MS => ⊥ end) σ'.2 Φ'.
+
+  
+  Lemma ewp_wrp_try_with E σ Φ σ' Φ' e h r :
+  EWPW e @ E <| σ |> {{ Φ }} -∗
+    shallow_handler_wrp E σ Φ h r σ' Φ' -∗
+      EWPW (TryWith e h r) @ E <| σ' |> {{ Φ' }}.
+  Proof.
+    iIntros "Hewp H". rewrite /shallow_handler_wrp /ewp_wrp. 
+    destruct σ.1 eqn:Hmd', σ'.1 eqn:Hmd;
+    iApply (ewp_try_with with "Hewp"); iApply "H".
+  Qed.
+
+  Definition deep_handler_wrp
+  (E : coPset)
+  (σ : sem_sig Σ)
+  (Φ : val -d> iProp Σ)
+  (h r : expr)
+  (σ' : sem_sig Σ)
+  (Φ' : val -d> iProp Σ) : iProp Σ :=
+    deep_handler E (match σ.1 with OS => σ.2 | MS => ⊥ end) σ.2 Φ h r
+                   (match σ'.1 with OS => σ'.2 | MS => ⊥ end) σ'.2 Φ'.
+
+  Lemma ewp_wrp_deep_try_with E σ Φ (h r : val) σ' Φ' e :
+  EWPW e @ E <| σ |> {{ Φ }} -∗
+    deep_handler_wrp E σ Φ h r σ' Φ' -∗
+      EWPW DeepTryWithV e h r @ E <| σ' |> {{ Φ' }}.
+  Proof.
+    iIntros "Hewp H". rewrite /deep_handler_wrp /ewp_wrp. 
+    destruct σ.1 eqn:Hmd', σ'.1 eqn:Hmd;
+    iApply (ewp_deep_try_with with "Hewp"); iApply "H".
+  Qed.
+
+End reasoning.
