theories/logic/sem_env.v
@@ -14,89 +14,109 @@ From haffel.lang Require Import hazel.
 From haffel.lang Require Import subst_map.
 From haffel.logic Require Import iEff.
 From haffel.logic Require Import sem_def.
-From haffel.logic Require Import sem_types.
 
-Lemma env_dom_nil {Σ} :
-  env_dom (Σ:= Σ) [] = [].
-Proof. done. Qed.
+Section env_lemmas_base.
+  
+  Context {Σ : gFunctors}.
 
-Lemma env_dom_cons {Σ} x τ (Γ : env Σ) :
-  env_dom ((x, τ) :: Γ) = x :: env_dom Γ.
-Proof. done. Qed.
+  Implicit Types Γ Γ₁ Γ₂ Γ₃ Δ : env Σ.
+  Implicit Types τ τ₁ τ₂ : sem_ty Σ.
 
-Lemma env_dom_app {Σ} (Γ₁ Γ₂ : env Σ) :
-  env_dom (Γ₁ ++ Γ₂) = env_dom Γ₁ ++ env_dom Γ₂.
-Proof. by rewrite -map_app. Qed.
+  Lemma env_dom_nil :
+    env_dom (Σ:= Σ) [] = [].
+  Proof. done. Qed.
+  
+  Lemma env_dom_cons x τ Γ :
+    env_dom ((x, τ) :: Γ) = x :: env_dom Γ.
+  Proof. done. Qed.
+  
+  Lemma env_dom_app Γ₁ Γ₂ :
+    env_dom (Γ₁ ++ Γ₂) = env_dom Γ₁ ++ env_dom Γ₂.
+  Proof. by rewrite -map_app. Qed.
+  
+  Lemma env_sem_typed_empty vs : ⟦ ([] : env Σ) ⟧ vs = True%I.
+  Proof. done. Qed.
+  
+  Lemma env_sem_typed_cons  x τ Γ' vs : 
+      ⟦ (x, τ) :: Γ' ⟧ vs = ((∃ v, ⌜ vs !! x = Some v ⌝ ∗ τ v) ∗ ⟦ Γ' ⟧ vs)%I.
+  Proof. done. Qed.
+  
+  Lemma env_sem_typed_insert Γ vs (x : string) v :
+    x ∉ (env_dom Γ) →
+    ⟦ Γ ⟧ vs ⊣⊢ ⟦ Γ ⟧ (binder_insert x v vs).
+  Proof.
+    intros Helem. 
+    iInduction Γ as [|[y τ] Γ'] "IH";
+      first (iSplit; iIntros; by rewrite env_sem_typed_empty). 
+    rewrite !env_sem_typed_cons; iSplit; iIntros "Henv";
+    iDestruct ("Henv") as "((%w & %Hvs & Hw) & HΓ')".
+    assert (x ≠ y).
+    { rewrite env_dom_cons in Helem.
+      destruct (not_elem_of_cons (env_dom Γ') x y) as [[ ] _]; done. }
+    - iSplitL "Hw".
+      + iExists _. iIntros "{$Hw} !%". 
+        destruct (decide (y = x)) as [->|]. 
+        { destruct Helem. rewrite env_dom_cons. apply elem_of_list_here. }
+        by rewrite lookup_insert_ne.
+      + iApply "IH"; last done. iPureIntro. 
+        destruct (not_elem_of_cons (env_dom Γ') x y) as [[ ] _]; done.
+    - iSplitL "Hw".
+      + iExists w.  iIntros "{$Hw} !%". 
+        destruct (decide (y = x)) as [->|]. 
+        { destruct Helem. rewrite env_dom_cons. apply elem_of_list_here. }
+        by rewrite lookup_insert_ne in Hvs.
+      + iApply "IH"; last done. iPureIntro. 
+        destruct (not_elem_of_cons (env_dom Γ') x y) as [[ ] _]; done.
+  Qed.
+  
+  Lemma env_sem_typed_delete Γ vs (x : string) :
+    x ∉ (env_dom Γ) →
+    ⟦ Γ ⟧ vs ⊣⊢ ⟦ Γ ⟧ (binder_delete x vs).
+  Proof.
+    intros Helem. 
+    iInduction Γ as [|[y τ] Γ'] "IH";
+      first (iSplit; iIntros; by rewrite env_sem_typed_empty). 
+    rewrite !env_sem_typed_cons; iSplit; iIntros "Henv";
+    iDestruct ("Henv") as "((%w & %Hvs & Hw) & HΓ')".
+    assert (x ≠ y).
+    { rewrite env_dom_cons in Helem.
+      destruct (not_elem_of_cons (env_dom Γ') x y) as [[ ] _]; done. }
+    - iSplitL "Hw".
+      + iExists _. iIntros "{$Hw} !% /=". 
+        by rewrite lookup_delete_ne.
+      + iApply "IH"; last done. iPureIntro. 
+        destruct (not_elem_of_cons (env_dom Γ') x y) as [[ ] _]; done.
+    - iSplitL "Hw".
+      + iExists w.  iIntros "{$Hw} !%". 
+        destruct (decide (y = x)) as [->|]. 
+        { destruct Helem. rewrite env_dom_cons. apply elem_of_list_here. }
+        simpl in Hvs.
+        by rewrite lookup_delete_ne in Hvs.
+      + iApply "IH"; last done. iPureIntro. 
+        destruct (not_elem_of_cons (env_dom Γ') x y) as [[ ] _]; done.
+  Qed.
+  
+  Lemma env_sem_typed_app Γ₁ Γ₂ vs :
+    ⟦ Γ₁ ++ Γ₂ ⟧ vs ⊣⊢ ⟦ Γ₁ ⟧ vs ∗ ⟦ Γ₂ ⟧ vs.
+  Proof. 
+    iInduction Γ₁ as [|[y τ] Γ₁'] "IH". 
+    { iSplit; [iIntros; by iFrame|iIntros "[_ H] {$H}"]. }
+    iSplit; rewrite !env_sem_typed_cons; iIntros "HΓ₁₂". 
+    - iDestruct "HΓ₁₂" as "($ & HΓ₁'₂)". by iApply "IH".
+    - iDestruct ("HΓ₁₂") as "[[Hτ HΓ₁'] HΓ₂]".
+      rewrite -/app. iFrame. iApply ("IH" with "[HΓ₁' HΓ₂]").
+      iFrame.
+  Qed.
 
-Lemma env_sem_typed_empty `{irisGS eff_lang Σ} vs : ⟦ [] ⟧ vs = True%I.
-Proof. done. Qed.
+End env_lemmas_base.
 
-Lemma env_sem_typed_cons `{irisGS eff_lang Σ} x τ Γ' vs : 
-    ⟦ (x, τ) :: Γ' ⟧ vs = ((∃ v, ⌜ vs !! x = Some v ⌝ ∗ τ v) ∗ ⟦ Γ' ⟧ vs)%I.
-Proof. done. Qed.
-
-Lemma env_sem_typed_insert `{irisGS eff_lang Σ} Γ vs (x : string) v :
-  x ∉ (env_dom Γ) →
-  ⟦ Γ ⟧ vs ⊣⊢ ⟦ Γ ⟧ (binder_insert x v vs).
-Proof.
-  intros Helem. 
-  iInduction Γ as [|[y τ] Γ'] "IH";
-    first (iSplit; iIntros; by rewrite env_sem_typed_empty). 
-  rewrite !env_sem_typed_cons; iSplit; iIntros "Henv";
-  iDestruct ("Henv") as "((%w & %Hvs & Hw) & HΓ')".
-  assert (x ≠ y).
-  { rewrite env_dom_cons in Helem.
-    destruct (not_elem_of_cons (env_dom Γ') x y) as [[ ] _]; done. }
-  - iSplitL "Hw".
-    + iExists _. iIntros "{$Hw} !%". 
-      destruct (decide (y = x)) as [->|]. 
-      { destruct Helem. rewrite env_dom_cons. apply elem_of_list_here. }
-      by rewrite lookup_insert_ne.
-    + iApply "IH"; last done. iPureIntro. 
-      destruct (not_elem_of_cons (env_dom Γ') x y) as [[ ] _]; done.
-  - iSplitL "Hw".
-    + iExists w.  iIntros "{$Hw} !%". 
-      destruct (decide (y = x)) as [->|]. 
-      { destruct Helem. rewrite env_dom_cons. apply elem_of_list_here. }
-      by rewrite lookup_insert_ne in Hvs.
-    + iApply "IH"; last done. iPureIntro. 
-      destruct (not_elem_of_cons (env_dom Γ') x y) as [[ ] _]; done.
-Qed.
-
-Lemma env_sem_typed_delete `{irisGS eff_lang Σ} Γ vs (x : string) :
-  x ∉ (env_dom Γ) →
-  ⟦ Γ ⟧ vs ⊣⊢ ⟦ Γ ⟧ (binder_delete x vs).
-Proof.
-  intros Helem. 
-  iInduction Γ as [|[y τ] Γ'] "IH";
-    first (iSplit; iIntros; by rewrite env_sem_typed_empty). 
-  rewrite !env_sem_typed_cons; iSplit; iIntros "Henv";
-  iDestruct ("Henv") as "((%w & %Hvs & Hw) & HΓ')".
-  assert (x ≠ y).
-  { rewrite env_dom_cons in Helem.
-    destruct (not_elem_of_cons (env_dom Γ') x y) as [[ ] _]; done. }
-  - iSplitL "Hw".
-    + iExists _. iIntros "{$Hw} !% /=". 
-      by rewrite lookup_delete_ne.
-    + iApply "IH"; last done. iPureIntro. 
-      destruct (not_elem_of_cons (env_dom Γ') x y) as [[ ] _]; done.
-  - iSplitL "Hw".
-    + iExists w.  iIntros "{$Hw} !%". 
-      destruct (decide (y = x)) as [->|]. 
-      { destruct Helem. rewrite env_dom_cons. apply elem_of_list_here. }
-      simpl in Hvs.
-      by rewrite lookup_delete_ne in Hvs.
-    + iApply "IH"; last done. iPureIntro. 
-      destruct (not_elem_of_cons (env_dom Γ') x y) as [[ ] _]; done.
-Qed.
-
-Ltac solve_sem_typed_insert :=
+Global Ltac solve_sem_typed_insert :=
   rewrite env_sem_typed_insert; try (simplify_eq; done); progress iFrame "%#∗".
 
-Ltac solve_sem_typed_insert_inv :=
+Global Ltac solve_sem_typed_insert_inv :=
   rewrite -env_sem_typed_insert; try (simplify_eq; done); progress iFrame "%#∗".
 
-Ltac solve_env := 
+Global Ltac solve_env := 
   repeat (
     done ||
     iIntros || 
@@ -113,133 +133,216 @@ Ltac solve_env :=
     solve_sem_typed_insert ||
     solve_sem_typed_insert_inv
   ).
+  
+Section env_lemmas_set_operations.
 
-Lemma env_sem_typed_union `{irisGS eff_lang Σ} Γ ws vs :
-  ⟦ Γ ⟧ vs ⊢ ⟦ Γ ⟧ (vs ∪ ws).
-Proof. 
-  iIntros "HΓ". iInduction Γ as [|[x τ] Γ'] "IH"; first done.
-  rewrite !env_sem_typed_cons.
-  iDestruct "HΓ" as "[(%m & %Hrw & Hx) HΓ']".
-  rewrite -/env_sem_typed. 
-  iSplitL "Hx"; [|by iApply "IH"].
-  iExists m; iFrame; iPureIntro.
-  by apply lookup_union_Some_l.
-Qed.
+  Context {Σ : gFunctors}.
 
-Lemma env_sem_typed_delete_union `{irisGS eff_lang Σ} Γ (Δ : env Σ) ws vs :
-  env_dom Γ ⊆ env_dom Δ →
-  ⟦ Γ ⟧ vs ⊣⊢ ⟦ Γ ⟧ (delete (env_dom Δ) ws ∪ vs).
-Proof.
-  intros ?. iSplit.
-  - iInduction Γ as [|[x τ] Γ'] "IH"; first solve_env. 
+  Implicit Types Γ Γ₁ Γ₂ Γ₃ Δ : env Σ.
+  Implicit Types τ τ₁ τ₂ : sem_ty Σ.
+
+  Lemma env_sem_typed_union Γ ws vs :
+    ⟦ Γ ⟧ vs ⊢ ⟦ Γ ⟧ (vs ∪ ws).
+  Proof. 
+    iIntros "HΓ". iInduction Γ as [|[x τ] Γ'] "IH"; first done.
     rewrite !env_sem_typed_cons.
-    iIntros "/= [(%w & %Hrw & Hw) HΓ']".
-    assert (Hseq' : env_dom Γ' ⊆ env_dom Δ). 
+    iDestruct "HΓ" as "[(%m & %Hrw & Hx) HΓ']".
+    rewrite -/env_sem_typed. 
+    iSplitL "Hx"; [|by iApply "IH"].
+    iExists m; iFrame; iPureIntro.
+    by apply lookup_union_Some_l.
+  Qed.
+  
+  Lemma env_sem_typed_delete_union Γ Δ ws vs :
+    env_dom Γ ⊆ env_dom Δ →
+    ⟦ Γ ⟧ vs ⊣⊢ ⟦ Γ ⟧ (delete (env_dom Δ) ws ∪ vs).
+  Proof.
+    intros ?. iSplit.
+    - iInduction Γ as [|[x τ] Γ'] "IH"; first solve_env. 
+      rewrite !env_sem_typed_cons.
+      iIntros "/= [(%w & %Hrw & Hw) HΓ']".
+      assert (Hseq' : env_dom Γ' ⊆ env_dom Δ). 
+      { eapply subset_cons. by erewrite <- env_dom_cons. }
+      assert (x ∈ (env_dom Δ)).
+      { eapply subset_cons_elem. by erewrite <- env_dom_cons. }
+      iSplitL "Hw";[| iApply ("IH" with "[] HΓ'"); by iPureIntro].
+      iExists w. iFrame. iPureIntro. 
+      rewrite (delete_list_elem_of _ x); last done.
+      rewrite lookup_union_r; first done. apply lookup_delete.
+    - iInduction Γ as [|[x τ] Γ'] "IH"; first solve_env.
+      rewrite !env_sem_typed_cons.
+      iIntros "[(%v & %Hrw & Hτ) HΓ']".
+      iSplitL "Hτ".
+      + iExists v. iIntros "{$Hτ} !%".
+        rewrite -(lookup_union_r (delete (env_dom Δ) ws)); first done.
+        rewrite (delete_list_elem_of _ x); first (apply lookup_delete).
+        eapply subset_cons_elem. by erewrite <- env_dom_cons.
+      + iApply "IH"; last done.
+        iPureIntro. eapply subset_cons. by erewrite <- env_dom_cons.
+  Qed.
+  
+  Lemma env_sem_typed_difference_delete Γ Δ vs ws :
+    env_dom Γ ⊆ env_dom Δ → ⟦ Γ ⟧ vs ⊣⊢ ⟦ Γ ⟧ (vs ∖ delete (env_dom Δ) ws).
+  Proof.
+    intros ?.
+    iInduction Γ as [|[x τ] Γ'] "IH"; first (iSplit; solve_env).
+    rewrite !env_sem_typed_cons; iSplit;
+    iIntros "/= [(%v & %Hrw & Hτ) HΓ']".
+    assert (Hseq' : env_dom Γ' ⊆ env_dom Δ).
     { eapply subset_cons. by erewrite <- env_dom_cons. }
     assert (x ∈ (env_dom Δ)).
     { eapply subset_cons_elem. by erewrite <- env_dom_cons. }
-    iSplitL "Hw";[| iApply ("IH" with "[] HΓ'"); by iPureIntro].
-    iExists w. iFrame. iPureIntro. 
-    rewrite (delete_list_elem_of _ x); last done.
-    rewrite lookup_union_r; first done. apply lookup_delete.
-  - iInduction Γ as [|[x τ] Γ'] "IH"; first solve_env.
+    - iSplitL "Hτ".
+      + iExists _. iFrame. iPureIntro. 
+        rewrite (delete_list_elem_of _ x); last done. 
+        by rewrite lookup_difference_delete. 
+      + iApply ("IH" with "[] HΓ'"); eauto. 
+    - iSplitL "Hτ".
+      + iExists _. iFrame. iPureIntro. 
+        rewrite (delete_list_elem_of _ x) in Hrw; 
+          [|eapply subset_cons_elem; by erewrite <- env_dom_cons].
+        by rewrite lookup_difference_delete in Hrw.
+      + iApply ("IH" with "[] HΓ'"); eauto. 
+        iPureIntro. eapply subset_cons. by erewrite <- env_dom_cons.
+  Qed.
+  
+  Lemma env_sem_typed_delete_disjoint Γ Δ vs  :
+    env_dom Γ ## env_dom Δ → ⟦ Γ ⟧ vs ⊣⊢ ⟦ Γ ⟧ (delete (env_dom Δ) vs).
+  Proof. 
+    iIntros (?).
+    iInduction Γ as [|[x τ] Γ'] "IH"; first (iSplit; solve_env). 
+    rewrite !env_sem_typed_cons; iSplit;
+    iIntros "/= [(%v & %Hrw & Hτ) HΓ']";
+    assert (Hseq' : env_dom Γ' ## env_dom Δ)
+      by (eapply disjoint_cons; by erewrite <- env_dom_cons);
+    assert (x ∉ (env_dom Δ)) by 
+      (eapply disjoint_cons_not_elem; by erewrite <- env_dom_cons).
+    - iSplitL "Hτ".
+      + iExists v. iIntros "{$Hτ} !%".
+        by rewrite lookup_delete_not_elem.
+      + by iApply "IH".
+    - iSplitL "Hτ".
+      + iExists v. iIntros "{$Hτ} !%".
+        by rewrite lookup_delete_not_elem in Hrw.
+      + by iApply "IH".
+  Qed. 
+  
+  Lemma env_sem_typed_union_difference_delete Γ Δ vs ws :
+    env_dom Γ ## env_dom Δ → ⟦ Γ ⟧ (vs ∪ ws ∖ (delete (env_dom Δ) ws)) ⊢ ⟦ Γ ⟧ vs.
+  Proof. 
+    intros ?.
+    iInduction Γ as [|[x τ] Γ'] "IH"; first solve_env.
     rewrite !env_sem_typed_cons.
-    iIntros "[(%v & %Hrw & Hτ) HΓ']".
+    iIntros "/= [(%v & %Hrw & Hτ) HΓ']".
+    assert (Hseq' : env_dom Γ' ## env_dom Δ)
+      by (eapply disjoint_cons; by erewrite <- env_dom_cons).
+    assert (x ∉ (env_dom Δ)) by 
+      (eapply disjoint_cons_not_elem; by erewrite <- env_dom_cons).
     iSplitL "Hτ".
     + iExists v. iIntros "{$Hτ} !%".
-      rewrite -(lookup_union_r (delete (env_dom Δ) ws)); first done.
-      rewrite (delete_list_elem_of _ x); first (apply lookup_delete).
-      eapply subset_cons_elem. by erewrite <- env_dom_cons.
-    + iApply "IH"; last done.
-      iPureIntro. eapply subset_cons. by erewrite <- env_dom_cons.
-Qed.
-
-Lemma env_sem_typed_difference_delete `{irisGS eff_lang Σ} Γ (Δ : env Σ) vs ws :
-  env_dom Γ ⊆ env_dom Δ → ⟦ Γ ⟧ vs ⊣⊢ ⟦ Γ ⟧ (vs ∖ delete (env_dom Δ) ws).
-Proof.
-  intros ?.
-  iInduction Γ as [|[x τ] Γ'] "IH"; first (iSplit; solve_env).
-  rewrite !env_sem_typed_cons; iSplit;
-  iIntros "/= [(%v & %Hrw & Hτ) HΓ']".
-  assert (Hseq' : env_dom Γ' ⊆ env_dom Δ).
-  { eapply subset_cons. by erewrite <- env_dom_cons. }
-  assert (x ∈ (env_dom Δ)).
-  { eapply subset_cons_elem. by erewrite <- env_dom_cons. }
-  - iSplitL "Hτ".
-    + iExists _. iFrame. iPureIntro. 
-      rewrite (delete_list_elem_of _ x); last done. 
-      by rewrite lookup_difference_delete. 
-    + iApply ("IH" with "[] HΓ'"); eauto. 
-  - iSplitL "Hτ".
-    + iExists _. iFrame. iPureIntro. 
-      rewrite (delete_list_elem_of _ x) in Hrw; 
-        [|eapply subset_cons_elem; by erewrite <- env_dom_cons].
-      by rewrite lookup_difference_delete in Hrw.
-    + iApply ("IH" with "[] HΓ'"); eauto. 
-      iPureIntro. eapply subset_cons. by erewrite <- env_dom_cons.
-Qed.
-
-Lemma env_sem_typed_delete_disjoint `{irisGS eff_lang Σ} Γ (Δ : env Σ) vs  :
-  env_dom Γ ## env_dom Δ → ⟦ Γ ⟧ vs ⊣⊢ ⟦ Γ ⟧ (delete (env_dom Δ) vs).
-Proof. 
-  iIntros (?).
-  iInduction Γ as [|[x τ] Γ'] "IH"; first (iSplit; solve_env). 
-  rewrite !env_sem_typed_cons; iSplit;
-  iIntros "/= [(%v & %Hrw & Hτ) HΓ']";
-  assert (Hseq' : env_dom Γ' ## env_dom Δ)
-    by (eapply disjoint_cons; by erewrite <- env_dom_cons);
-  assert (x ∉ (env_dom Δ)) by 
-    (eapply disjoint_cons_not_elem; by erewrite <- env_dom_cons).
-  - iSplitL "Hτ".
-    + iExists v. iIntros "{$Hτ} !%".
-      by rewrite lookup_delete_not_elem.
+      by rewrite lookup_union_delete_disjoint in Hrw.
     + by iApply "IH".
-  - iSplitL "Hτ".
-    + iExists v. iIntros "{$Hτ} !%".
-      by rewrite lookup_delete_not_elem in Hrw.
-    + by iApply "IH".
-Qed. 
+  Qed.
+  
+End env_lemmas_set_operations.
 
-Lemma env_sem_typed_union_difference_delete `{irisGS eff_lang Σ} Γ (Δ : env Σ) vs ws :
-  env_dom Γ ## env_dom Δ → ⟦ Γ ⟧ (vs ∪ ws ∖ (delete (env_dom Δ) ws)) ⊢ ⟦ Γ ⟧ vs.
-Proof. 
-  intros ?.
-  iInduction Γ as [|[x τ] Γ'] "IH"; first solve_env.
-  rewrite !env_sem_typed_cons.
-  iIntros "/= [(%v & %Hrw & Hτ) HΓ']".
-  assert (Hseq' : env_dom Γ' ## env_dom Δ)
-    by (eapply disjoint_cons; by erewrite <- env_dom_cons).
-  assert (x ∉ (env_dom Δ)) by 
-    (eapply disjoint_cons_not_elem; by erewrite <- env_dom_cons).
-  iSplitL "Hτ".
-  + iExists v. iIntros "{$Hτ} !%".
-    by rewrite lookup_union_delete_disjoint in Hrw.
-  + by iApply "IH".
-Qed.
+Section env_sub_typing.
 
-Lemma env_sem_typed_app `{irisGS eff_lang Σ} Γ₁ Γ₂ vs :
-  ⟦ Γ₁ ++ Γ₂ ⟧ vs ⊣⊢ ⟦ Γ₁ ⟧ vs ∗ ⟦ Γ₂ ⟧ vs.
-Proof. 
-  iInduction Γ₁ as [|[y τ] Γ₁'] "IH". 
-  { iSplit; [iIntros; by iFrame|iIntros "[_ H] {$H}"]. }
-  iSplit; rewrite !env_sem_typed_cons; iIntros "HΓ₁₂". 
-  - iDestruct "HΓ₁₂" as "($ & HΓ₁'₂)". by iApply "IH".
-  - iDestruct ("HΓ₁₂") as "[[Hτ HΓ₁'] HΓ₂]".
-    rewrite -/app. iFrame. iApply ("IH" with "[HΓ₁' HΓ₂]").
-    iFrame.
-Qed.
+  Context {Σ : gFunctors}.
 
-Lemma env_sem_typed_mk_moved `{irisGS eff_lang Σ} vs Γ :
-  ⟦ Γ ⟧ vs -∗
-  □ ⟦ map (prod_map id (const Moved)) Γ ⟧ vs ∗ ⟦ Γ ⟧ vs.
-Proof.
-  iIntros "HΓ". iInduction Γ as [|x Γ'] "IH"; first done. simpl.
-  destruct x. simpl. rewrite !env_sem_typed_cons.
-  iDestruct "HΓ" as "[(%w & -> & Hw) HΓ']". 
-  iSpecialize ("IH" with "HΓ'"). 
-  rewrite bi.intuitionistically_sep.
-  rewrite -bi.sep_assoc. iSplitR.
-  { by iExists w. }
-  iDestruct "IH" as "[HΓ'T HΓ']". iFrame.
-  { iExists w. by iFrame. }
-Qed.
+  Implicit Types Γ Γ₁ Γ₂ Γ₃ : env Σ.
+  Implicit Types τ τ₁ τ₂ : sem_ty Σ.
+
+  Lemma env_le_refl Γ : ⊢ Γ ≤E Γ.
+  Proof. iIntros "!# % $". Qed.
+  
+  Lemma env_le_trans Γ₁ Γ₂ Γ₃ : 
+    Γ₁ ≤E Γ₂ -∗
+    Γ₂ ≤E Γ₃ -∗
+    Γ₁ ≤E Γ₃.
+  Proof.
+    iIntros "#HΓ₁₂ #HΓ₂₃ !# %vs HΓ₁ //=".  
+    iApply "HΓ₂₃". by iApply "HΓ₁₂".
+  Qed.
+  
+  Lemma env_le_cons Γ₁ Γ₂ τ₁ τ₂ x :
+    Γ₁ ≤E Γ₂ -∗
+    τ₁ ≤T τ₂ -∗
+    (x, τ₁) :: Γ₁ ≤E (x, τ₂) :: Γ₂.
+  Proof.
+    iIntros "#HΓ₁₂ #Hτ₁₂ !# %vs [%v (Hlookup & Hv & HΓ₁)]".
+    iExists v. iFrame. iSplitR "HΓ₁"; last (by iApply "HΓ₁₂").
+    by iApply "Hτ₁₂".
+  Qed.
+  
+  Lemma env_le_copy_contraction Γ x τ :
+    copy_ty τ -∗
+    (x, τ) :: Γ ≤E (x, τ) :: (x, τ) :: Γ.
+  Proof.
+    iIntros "#Hcpy !# %vs".
+    iIntros "//= [%w (%Hrw & Hτ & HΓ)]". 
+    iDestruct ("Hcpy" with "Hτ") as "#Hτ'".
+    by do 2 (iExists w; iFrame "%#").
+  Qed.
+  
+  Lemma env_le_bring_forth Γ n x τ :
+    nth_error Γ n = Some (x, τ) →
+    ⊢ Γ ≤E (x, τ) :: (list_delete n Γ) .
+  Proof.
+    iInduction n as [|] "IH" forall (Γ); iIntros (Hnth vs);
+    iIntros "!# HΓ"; simpl in Hnth; destruct Γ; first done; simplify_eq; first done.
+    destruct p; simpl. rewrite !env_sem_typed_cons.
+    iDestruct "HΓ" as "[$ HΓ]". rewrite -env_sem_typed_cons.
+    by iApply "IH". 
+  Qed.
+  
+  Lemma env_le_bring_forth_rev Γ n x τ :
+    nth_error Γ n = Some (x, τ) →
+    ⊢ (x, τ) :: (list_delete n Γ) ≤E Γ.
+  Proof.
+    iInduction n as [|] "IH" forall (Γ); iIntros (Hnth vs);
+    simpl in Hnth; 
+    destruct Γ as [|[y κ] Γ']; first done; 
+    simplify_eq; simpl; first (iIntros "!# $").
+    iIntros "!# [%v (? & ? & [%w (? & ? & ?)])]". 
+    iExists w. iFrame. iApply "IH"; first done.
+    iExists v. iFrame.
+  Qed.
+  
+  Lemma env_le_swap_second Γ x y τ₁ τ₂ : 
+    ⊢ (y, τ₂) :: (x, τ₁) :: Γ ≤E (x, τ₁) :: (y, τ₂) :: Γ.
+  Proof.
+    pose proof (env_le_bring_forth_rev ((x, τ₁) :: (y, τ₂) :: Γ) 1 y τ₂).
+    by apply H.
+  Qed.
+  
+  Lemma env_le_swap_third Γ x y z τ₁ τ₂ τ₃: 
+    ⊢ (z, τ₃) :: (x, τ₁) :: (y, τ₂) :: Γ ≤E (x, τ₁) :: (y, τ₂) :: (z, τ₃) :: Γ.
+  Proof.
+    pose proof (env_le_bring_forth_rev ((x, τ₁) :: (y, τ₂) :: (z, τ₃) :: Γ) 2 z τ₃).
+    by apply H.
+  Qed.
+  
+  Lemma env_le_swap_fourth Γ x y z z' τ₁ τ₂ τ₃ τ₄: 
+    ⊢ (z', τ₄) :: (x, τ₁) :: (y, τ₂) :: (z, τ₃) :: Γ ≤E (x, τ₁) :: (y, τ₂) :: (z, τ₃) :: (z', τ₄) :: Γ.
+  Proof.
+    pose proof (env_le_bring_forth_rev ((x, τ₁) :: (y, τ₂) :: (z, τ₃) :: (z', τ₄) :: Γ) 3 z' τ₄).
+    by apply H.
+  Qed.
+  
+  Lemma env_le_swap_env_singl Γ x τ : 
+    ⊢ (x, τ) :: Γ ≤E Γ ++ [(x, τ)].
+  Proof.
+    induction Γ as [|[y κ] Γ'].
+    { simpl. iIntros "!# % $". }
+    rewrite -app_comm_cons.
+    iApply env_le_trans; [iApply env_le_swap_second|].
+    iApply env_le_cons; last (iIntros "!# % $").
+    iApply IHΓ'.
+  Qed.
+  
+  Lemma env_le_weaken Γ x τ :
+    ⊢ (x, τ) :: Γ ≤E Γ.
+  Proof. iIntros "!# % [% (? & ? & $)]". Qed.
+
+End env_sub_typing.
