theories/logic/sem_judgement.v
@@ -1,0 +1,66 @@
+
+(* sem_judgements.v *)
+
+(* This file contains the definition of semantic typing judgments.
+*)
+
+From iris.proofmode Require Import base tactics classes.
+From iris.algebra Require Import list.
+From iris.program_logic Require Import weakestpre.
+
+From stdpp Require Import base gmap.
+
+(* Hazel Reasoning *)
+From hazel.program_logic Require Import weakest_precondition
+                                        state_reasoning.
+
+(* Local imports *)
+From haffel.lib Require Import base.
+From haffel.lang Require Import hazel.
+From haffel.lang Require Import subst_map.
+From haffel.logic Require Import iEff.
+From haffel.logic Require Import sem_def.
+From haffel.logic Require Import ewp_wrp.
+
+(* Semantic typing judgment. *)
+
+(* The semantic typing judgment is defined to be persistent
+ * because we want the persistent resources it uses to only be 
+ * from the environment Γ.
+ *)
+Definition sem_typed `{!heapGS Σ}
+  (Γ₁ : env Σ)
+  (e : expr)
+  (σ : sem_sig Σ)
+  (τ : sem_ty Σ) 
+  (Γ₂ : env Σ) : iProp Σ :=
+    tc_opaque (□ (∀ (vs : gmap string val),
+                    env_sem_typed Γ₁ vs -∗ 
+                    (EWPW (subst_map vs e) <| σ |> {{ v, τ v ∗ env_sem_typed Γ₂ vs }})))%I.
+
+Global Instance sem_typed_persistent `{!heapGS Σ} (Γ Γ' : env Σ) e σ τ :
+  Persistent (sem_typed Γ e σ τ Γ').
+Proof.
+  unfold sem_typed, tc_opaque. apply _.
+Qed.
+
+Notation "Γ₁ ⊨ e : σ : α ⊨ Γ₂" := (sem_typed Γ₁ e%E σ%S α%T Γ₂)
+  (at level 74, e, σ, α at next level) : bi_scope.
+
+Notation "⊨ e : σ : α" := (sem_typed [] e%E σ%S α%T [])
+  (at level 74, e, σ, α at next level) : bi_scope.
+
+(* The value semantic typing judgement is also defined
+ * to be persistent, so only persistent values hold for it.
+ *) 
+Definition sem_val_typed `{!irisGS eff_lang Σ} 
+  (v : val) 
+  (A : sem_ty Σ) : iProp Σ := tc_opaque (□ (A v))%I.
+
+Notation "⊨ᵥ v : τ" := (sem_val_typed v%V τ%T)
+  (at level 20, v, τ at next level) : bi_scope.
+Global Instance sem_typed_val_persistent `{!irisGS eff_lang Σ} v τ :
+  Persistent (sem_val_typed v τ).
+Proof.
+  unfold sem_val_typed, tc_opaque. apply _.
+Qed.
