theories/logic/sem_sig.v
@@ -1,0 +1,204 @@
+(* sem_sig.v *)
+
+(* This file contains the definition of semantic types and signatures,
+   together with the definition of base types and type formers.  
+*)
+
+From iris.proofmode Require Import base tactics.
+From iris.algebra Require Import ofe list.
+From iris.base_logic Require Export iprop upred invariants.
+
+(* Hazel Reasoning *)
+From hazel.program_logic Require Import weakest_precondition 
+                                        state_reasoning
+                                        protocols.
+
+(* Local imports *)
+From haffel.lib Require Import logic.
+From haffel.lang Require Import hazel.
+From haffel.lang Require Import subst_map.
+From haffel.logic Require Import iEff.
+From haffel.logic Require Import sem_def.
+
+(* Empty Effect Signature *)
+Definition sem_sig_nil {Σ} : sem_sig Σ := (inhabitant, iEff_bottom).
+Global Instance Bottom {Σ} : Bottom (sem_sig Σ) := sem_sig_nil.
+
+Lemma sem_sig_bot_ieff {Σ} (σ : sem_sig Σ) : 
+    σ ≤S ⊥ -∗ iEff_le σ.2 ⊥.
+Proof. iIntros "[$|[_ $]]". Qed.
+
+Lemma sem_sig_to_ieff {Σ} (σ σ' : sem_sig Σ) : 
+    σ ≤S σ' -∗ iEff_le σ.2 σ'.2.
+Proof. 
+  iIntros "[Hbot|[_ $]]". 
+  iApply (iEff_le_trans with "Hbot"). iApply iEff_le_bottom.
+Qed.
+
+(* Universally Quantified, Recursive Effect Signature *)
+
+(* Effect Signature *)
+Definition sem_sig_eff_rec_pre {Σ} m (A B : sem_sig Σ -d> sem_ty Σ -d> sem_ty Σ) (rec : sem_sig Σ) : sem_sig Σ :=
+  (m, >> (α : sem_ty Σ) (a : val) >> ! a {{ ▷ (∃ rec', rec ≡ rec' ∧ A rec' α a) }}; 
+      << (b : val)                << ? b {{ ▷ (∃ rec', rec ≡ rec' ∧ B rec' α b) }} @m)%ieff.
+
+Global Instance sem_sig_eff_rec_pre_contractive {Σ} m (A B : sem_sig Σ -d> sem_ty Σ -d> sem_ty Σ) :
+  Contractive (sem_sig_eff_rec_pre m A B).
+Proof.
+  intros ????.
+  rewrite /sem_sig_eff_rec_pre iEffPre_exist_eq iEffPost_exist_eq /=. f_equiv.
+  intros ??. simpl. do 3 f_equiv. rewrite iEffPre_base_eq /=.
+  intros ?. simpl. do 2 f_equiv.
+  { f_contractive. simpl in H. by do 4 f_equiv. }
+  do 2 f_equiv. rewrite /iEffPost_exist_def. do 3 f_equiv.
+  rewrite iEffPost_base_eq /iEffPost_base_def. do 2 f_equiv. f_contractive.
+  simpl in H. by do 4 f_equiv.
+Qed.
+
+Definition sem_sig_eff_rec {Σ} m (A B : sem_sig Σ → sem_ty Σ → sem_ty Σ) : sem_sig Σ :=
+  fixpoint (sem_sig_eff_rec_pre m A B).
+
+Lemma sem_sig_eff_rec_unfold {Σ} m (A B : sem_sig Σ → sem_ty Σ → sem_ty Σ) `{NonExpansive2 A, NonExpansive2 B} :
+  (sem_sig_eff_rec m A B) ≡ 
+    (m, >> (α : sem_ty Σ) (a : val) >> ! a {{ ▷ (A (sem_sig_eff_rec m A B) α a) }}; 
+        << (b : val)                << ? b {{ ▷ (B (sem_sig_eff_rec m A B) α b) }} @m)%ieff.
+Proof.
+  rewrite {1} /sem_sig_eff_rec fixpoint_unfold {1} /sem_sig_eff_rec_pre.
+  do 6 f_equiv. 
+  - iSplit. 
+    + iIntros "[% [#Hfix HA]] !>". 
+      rewrite /sem_sig_eff_rec.
+      iAssert (A rec' a ≡ A (fixpoint (sem_sig_eff_rec_pre m A B)) a)%I as "#H".
+      { by iRewrite "Hfix". }
+      rewrite discrete_fun_equivI. by iRewrite - ("H" $! a0).
+    + iIntros "HA //=". iExists (sem_sig_eff_rec m A B).
+      by iFrame. 
+  - intros ?. rewrite iEffPost_base_eq /iEffPost_base_def.
+    apply non_dep_fun_equiv. do 2 f_equiv. intros ?. do 2 f_equiv. iSplit.
+    + iIntros "[% [#Hfix HB]]". 
+      rewrite /sem_sig_eff_rec.
+      iAssert (B rec' a ≡ B (fixpoint (sem_sig_eff_rec_pre m A B)) a)%I as "#H".
+      { by iRewrite "Hfix". }
+      rewrite discrete_fun_equivI. by iRewrite - ("H" $! a1).
+    + iIntros "Hτ //=". iExists (sem_sig_eff_rec m A B).
+      by iFrame. 
+Qed.
+
+Lemma sem_sig_eff_rec_unfold_1 {Σ} m (A B : sem_sig Σ → sem_ty Σ → sem_ty Σ) `{NonExpansive2 A, NonExpansive2 B} :
+  (sem_sig_eff_rec m A B).1 ≡ m.
+Proof. by rewrite sem_sig_eff_rec_unfold. Qed.
+
+Lemma sem_sig_eff_rec_unfold_2 {Σ} m (A B : sem_sig Σ -d> sem_ty Σ -d> sem_ty Σ) `{ NonExpansive2 A, NonExpansive2 B } :
+  (sem_sig_eff_rec m A B).2 ≡
+    (>> (α : sem_ty Σ) (a : val) >> ! a {{ ▷ (A (sem_sig_eff_rec m A B) α a) }}; 
+     << (b : val)                << ? b {{ ▷ (B (sem_sig_eff_rec m A B) α b) }} @m)%ieff.
+Proof. by rewrite {1} sem_sig_eff_rec_unfold. Qed.
+
+Lemma sem_sig_eff_rec_unfold_iEff {Σ} m (A B : sem_sig Σ -d> sem_ty Σ -d> sem_ty Σ) `{ NonExpansive2 A, NonExpansive2 B } v Φ:
+  iEff_car (sem_sig_eff_rec m A B).2 v Φ ⊣⊢
+    iEff_car (>> (α : sem_ty Σ) (a : val) >> ! a {{ ▷ (A (sem_sig_eff_rec m A B) α a) }}; 
+              << (b : val)                << ? b {{ ▷ (B (sem_sig_eff_rec m A B) α b) }} @m)%ieff v Φ.
+Proof.
+  assert (Hequiv :
+  iEff_car (sem_sig_eff_rec m A B).2 v Φ ⊣⊢
+    iEff_car (>> (α : sem_ty Σ) (a : val) >> ! a {{ ▷ (A (sem_sig_eff_rec m A B) α a) }}; 
+              << (b : val)                << ? b {{ ▷ (B (sem_sig_eff_rec m A B) α b) }} @m)%ieff v Φ).
+  { f_equiv. apply non_dep_fun_equiv. by apply sem_sig_eff_rec_unfold. }
+  by rewrite Hequiv.
+Qed.
+
+Lemma sem_sig_eff_rec_eq {Σ} m A B v Φ `{ NonExpansive2 A, NonExpansive2 B }:
+  iEff_car (sem_sig_eff_rec (Σ:=Σ) m A B).2 v Φ ⊣⊢
+    (∃ α a, ⌜ a = v ⌝ ∗ (▷ A (sem_sig_eff_rec m A B) α a) ∗ 
+                        □? m (∀ b, (▷ B (sem_sig_eff_rec m A B) α b) -∗ Φ b))%I.
+Proof. 
+  etrans; [by apply sem_sig_eff_rec_unfold_iEff|]. 
+  by rewrite (iEff_tele_eq' [tele _ _] [tele _]) /=. 
+Qed.
+
+(* The sem_sig_eff_rec protocol is monotonic. *)
+Global Instance sem_sig_eff_rec_mono_prot {Σ} A B `{ NonExpansive2 A, NonExpansive2 B }:
+  MonoProt (@sem_sig_eff_rec Σ OS A B).2.
+Proof.
+  constructor. iIntros (???) "HΦ'".
+  rewrite !sem_sig_eff_rec_eq /=.
+  iIntros "(% & % & <- & Hτ & HκΦ)".
+  iExists α, a. iSplitR; first done. iFrame. simpl.
+  iIntros (b) "Hκ". iApply "HΦ'". by iApply "HκΦ".
+Qed.
+
+(* The sem_sig_eff_rec protocol is persistently monotonic. *)
+Global Instance sem_sig_eff_rec_pers_mono_prot {Σ} A B `{ NonExpansive2 A, NonExpansive2 B }:
+  PersMonoProt (@sem_sig_eff_rec Σ MS A B).2.
+Proof.
+  constructor. iIntros (???) "#HΦ'".
+  rewrite !sem_sig_eff_rec_eq. simpl.
+  iIntros "(% & % & <- & Hτ & #HκΦ)".
+  iExists α, a. iSplitR; first done. iFrame. simpl.
+  iIntros "!# %b Hκ". iApply "HΦ'". by iApply "HκΦ".
+Qed.
+
+Lemma upcl_sem_sig_rec_eff {Σ} m A B v Φ `{ NonExpansive2 A, NonExpansive2 B}:
+  iEff_car (upcl m (sem_sig_eff_rec (Σ:=Σ) m A B).2) v Φ ⊣⊢
+    (∃ α a, ⌜ a = v ⌝ ∗ (▷ A (sem_sig_eff_rec m A B) α a) ∗ 
+                        □? m (∀ b, (▷ B (sem_sig_eff_rec m A B) α b) -∗ Φ b))%I.
+Proof.
+  assert (Hequiv:
+    iEff_car (upcl m (sem_sig_eff_rec m A B).2) v Φ ≡ iEff_car (sem_sig_eff_rec m A B).2 v Φ).
+  { f_equiv. apply non_dep_fun_equiv. destruct m; [by rewrite upcl_id|by rewrite pers_upcl_id]. }
+  rewrite Hequiv. by apply sem_sig_eff_rec_eq.
+Qed.
+
+(* Notations. *)
+Notation "'μ∀TS:' θ , α , τ ⇒ κ | m " := (sem_sig_eff_rec m (λ θ α, τ%T) (λ θ α, κ%T))
+  (at level 100, m, τ, κ at level 200) : sem_sig_scope.
+
+(* Sub-Typing on Signatures *)
+
+Lemma sig_le_refl {Σ} (σ : sem_sig Σ) : ⊢ σ ≤S σ.
+Proof. iRight. iSplit;[by destruct σ.1, σ.2|iApply iEff_le_refl]. Qed.
+
+Lemma sig_le_trans {Σ} (σ₁ σ₂ σ₃: sem_sig Σ) : 
+    σ₁ ≤S σ₂ -∗
+    σ₂ ≤S σ₃ -∗
+    σ₁ ≤S σ₃. 
+Proof. 
+  iIntros "[#Hb₁₂|[#Hm₁₂ #Hp₁₂]] [#Hb₂₃|[#Hm₂₃ #Hp₂₃]]"; rewrite /sig_le /tc_opaque. 
+  - by iLeft.
+  - by iLeft.
+  - iLeft. iIntros (v Φ) "!# Hσ₁".
+    iApply "Hb₂₃". by iApply "Hp₁₂".
+  - iRight. 
+    iSplitL; [|iApply iEff_le_trans; [iApply "Hp₁₂"|iApply "Hp₂₃"]].
+    by destruct σ₁.1, σ₂.1, σ₃.1.
+Qed.
+
+Lemma sig_le_nil {Σ} (σ : sem_sig Σ) :
+  ⊢ ⊥ ≤S σ.
+Proof. iLeft. iApply iEff_le_bottom. Qed.
+
+Lemma sig_le_eff_rec {Σ} m₁ m₂ (ι₁ ι₂ κ₁ κ₂ : sem_sig Σ → sem_ty Σ → sem_ty Σ)
+  `{NonExpansive2 ι₁, NonExpansive2 ι₂, NonExpansive2 κ₁, NonExpansive2 κ₂ } :
+  m₁ ≤M m₂ -∗
+  □ (∀ α σ σ', σ ≤S σ' -∗ (ι₁ σ α) ≤T (ι₂ σ' α)) -∗
+  □ (∀ α σ σ', σ ≤S σ' -∗ (κ₂ σ' α) ≤T (κ₁ σ α)) -∗
+  (μ∀TS: θ , α , ι₁ θ α ⇒ κ₁ θ α | m₁) ≤S (μ∀TS: θ , α , ι₂ θ α ⇒ κ₂ θ α | m₂).
+Proof.
+  iIntros "#mle #Hι₁₂ #Hκ₂₁". iLöb as "IH". 
+  iRight. iSplitL.
+  { by rewrite !sem_sig_eff_rec_unfold_1 /=. }
+  iIntros (v Φ) "!#".
+  rewrite !sem_sig_eff_rec_eq.
+  iIntros "(%α & %w & <- & Hι₁ & HκΦ₁)".
+  iExists α, w; iSplitR; first done.
+  iSplitL "Hι₁".
+  { iNext. iApply ("Hι₁₂" with "IH Hι₁"). }
+  simpl. destruct m₁, m₂; rewrite /mode_le /mode_le_prop; eauto; simpl.
+  - iIntros (b) "Hκ₂". iApply "HκΦ₁".
+    iNext. iApply ("Hκ₂₁" with "IH Hκ₂").
+  - iIntros (b) "Hκ₂". iApply "HκΦ₁".
+    iNext. iApply ("Hκ₂₁" with "IH Hκ₂").
+  - iDestruct "HκΦ₁" as "#HκΦ₁".
+    iIntros "!# %b Hκ₂". iApply "HκΦ₁".
+    iNext. iApply ("Hκ₂₁" with "IH Hκ₂").
+Qed.
